rocq/theories/TypeSystem/Types.v
@@ -16,6 +16,16 @@ Inductive ref_kind :=
 | RShared      (* &T *)
 | RUnique.     (* &mut T *)
 
+Record core_trait_ref (A : Type) : Type := MkCoreTraitRef {
+  core_trait_ref_name : string;
+  core_trait_ref_args : list A
+}.
+
+Record core_trait_bound (A : Type) : Type := MkCoreTraitBound {
+  core_bound_type_index : nat;
+  core_bound_traits     : list (core_trait_ref A)
+}.
+
 Inductive TypeCore (A : Type) : Type :=
 | TUnits    : TypeCore A
 | TIntegers : TypeCore A
@@ -27,6 +37,7 @@ Inductive TypeCore (A : Type) : Type :=
 | TFn       : list A -> A -> TypeCore A
 | TClosure  : lifetime -> list A -> A -> TypeCore A
 | TForall   : nat -> outlives_ctx -> A -> TypeCore A
+| TTypeForall : nat -> list (core_trait_bound A) -> A -> TypeCore A
 | TRef      : lifetime -> ref_kind -> A -> TypeCore A.
 
 Arguments TUnits {A}.
@@ -39,6 +50,7 @@ Arguments TStruct {A} _ _ _.
 Arguments TFn {A} _ _.
 Arguments TClosure {A} _ _ _.
 Arguments TForall {A} _ _ _.
+Arguments TTypeForall {A} _ _ _.
 Arguments TRef {A} _ _ _.
 
 Inductive Ty : Type :=
@@ -83,6 +95,15 @@ Fixpoint apply_lt_lifetime (σ : list lifetime) (l : lifetime) : lifetime :=
 Definition apply_lt_outlives (σ : list lifetime) (Ω : outlives_ctx) : outlives_ctx :=
   map (fun '(a, b) => (apply_lt_lifetime σ a, apply_lt_lifetime σ b)) Ω.
 
+Definition map_core_trait_ref
+    {A B : Type} (f : A -> B) (tr : core_trait_ref A) : core_trait_ref B :=
+  MkCoreTraitRef B (core_trait_ref_name A tr) (map f (core_trait_ref_args A tr)).
+
+Definition map_core_trait_bound
+    {A B : Type} (f : A -> B) (b : core_trait_bound A) : core_trait_bound B :=
+  MkCoreTraitBound B (core_bound_type_index A b)
+    (map (map_core_trait_ref f) (core_bound_traits A b)).
+
 Definition close_fn_lifetime (m : nat) (l : lifetime) : lifetime :=
   match l with
   | LVar i => if Nat.ltb i m then LBound i else l
@@ -123,6 +144,8 @@ Fixpoint apply_lt_ty (σ : list lifetime) (T : Ty) {struct T} : Ty :=
       MkTy u (TClosure (apply_lt_lifetime σ l) (map_lt ts) (apply_lt_ty σ r))
   | MkTy u (TForall n Ω body) =>
       MkTy u (TForall n (apply_lt_outlives σ Ω) (apply_lt_ty σ body))
+  | MkTy u (TTypeForall n bounds body) =>
+      MkTy u (TTypeForall n bounds (apply_lt_ty σ body))
   | MkTy u (TRef l rk t) =>
       MkTy u (TRef (apply_lt_lifetime σ l) rk (apply_lt_ty σ t))
   end.
@@ -163,6 +186,8 @@ Fixpoint map_lifetimes_ty
   | MkTy u (TForall n Ω body) =>
       MkTy u (TForall n (map (fun '(a, b) => (f a, f b)) Ω)
         (map_lifetimes_ty f body))
+  | MkTy u (TTypeForall n bounds body) =>
+      MkTy u (TTypeForall n bounds (map_lifetimes_ty f body))
   | MkTy u (TRef l rk t) =>
       MkTy u (TRef (f l) rk (map_lifetimes_ty f t))
   end.
@@ -222,6 +247,7 @@ Proof.
       - reflexivity.
       - rewrite !close_fn_lifetime_0, IHrest. reflexivity. }
     rewrite Hbounds, IH. reflexivity.
+  - rewrite IH. reflexivity.
   - rewrite close_fn_lifetime_0, IH. reflexivity.
 Qed.
 
@@ -275,6 +301,8 @@ Fixpoint contains_lbound_ty (T : Ty) : bool :=
       contains_lbound_lifetime l || existsb contains_lbound_ty ts || contains_lbound_ty r
   | MkTy _ (TForall _ Ω body) =>
       contains_lbound_outlives Ω || contains_lbound_ty body
+  | MkTy _ (TTypeForall _ bounds body) =>
+      contains_lbound_ty body
   | MkTy _ (TRef l _ t) =>
       contains_lbound_lifetime l || contains_lbound_ty t
   | _ => false
@@ -289,6 +317,8 @@ Fixpoint ty_ref_free_b (T : Ty) : bool :=
   | MkTy _ (TClosure _ ts r) =>
       false
   | MkTy _ (TForall _ _ body) =>
+      ty_ref_free_b body
+  | MkTy _ (TTypeForall _ bounds body) =>
       ty_ref_free_b body
   | MkTy _ (TRef _ _ _) =>
       false
