rocq/theories/Validation/Validator.v
@@ -61,10 +61,11 @@ Fixpoint type_struct_refs (T : Ty) : list string :=
       fold_right (fun T acc => type_struct_refs T ++ acc) [] args
   | MkTy _ (TFn args ret) =>
       fold_right (fun T acc => type_struct_refs T ++ acc) (type_struct_refs ret) args
-  | MkTy _ (TClosure _ args ret) =>
-      fold_right (fun T acc => type_struct_refs T ++ acc) (type_struct_refs ret) args
-  | MkTy _ (TForall _ _ body) => type_struct_refs body
-  | MkTy _ (TRef _ _ inner) => type_struct_refs inner
+	  | MkTy _ (TClosure _ args ret) =>
+	      fold_right (fun T acc => type_struct_refs T ++ acc) (type_struct_refs ret) args
+	  | MkTy _ (TForall _ _ body) => type_struct_refs body
+	  | MkTy _ (TTypeForall _ _ body) => type_struct_refs body
+	  | MkTy _ (TRef _ _ inner) => type_struct_refs inner
   | _ => []
   end.
 
@@ -149,10 +150,12 @@ Fixpoint type_env_wf_b
       lifetime_wf_b lt_params bound_depth env_lt &&
       forallb (type_env_wf_b structs ty_params lt_params bound_depth) args &&
       type_env_wf_b structs ty_params lt_params bound_depth ret
-  | MkTy _ (TForall n Ω body) =>
-      outlives_wf_b lt_params (n + bound_depth) Ω &&
-      type_env_wf_b structs ty_params lt_params (n + bound_depth) body
-  | MkTy _ (TRef l _ inner) =>
+	  | MkTy _ (TForall n Ω body) =>
+	      outlives_wf_b lt_params (n + bound_depth) Ω &&
+	      type_env_wf_b structs ty_params lt_params (n + bound_depth) body
+	  | MkTy _ (TTypeForall n _ body) =>
+	      type_env_wf_b structs (n + ty_params) lt_params bound_depth body
+	  | MkTy _ (TRef l _ inner) =>
       lifetime_wf_b lt_params bound_depth l &&
       type_env_wf_b structs ty_params lt_params bound_depth inner
   end.
@@ -189,15 +192,16 @@ Fixpoint used_type_params_ty (T : Ty) : list nat :=
         | x :: rest => used_type_params_ty x ++ go rest
         end
       in go args
-  | MkTy _ (TClosure _ args ret) =>
-      let fix go (xs : list Ty) : list nat :=
+	  | MkTy _ (TClosure _ args ret) =>
+	      let fix go (xs : list Ty) : list nat :=
         match xs with
         | [] => used_type_params_ty ret
         | x :: rest => used_type_params_ty x ++ go rest
         end
-      in go args
-  | MkTy _ (TForall _ _ body) => used_type_params_ty body
-  | MkTy _ (TRef _ _ inner) => used_type_params_ty inner
+	      in go args
+	  | MkTy _ (TForall _ _ body) => used_type_params_ty body
+	  | MkTy _ (TTypeForall _ _ body) => used_type_params_ty body
+	  | MkTy _ (TRef _ _ inner) => used_type_params_ty inner
   | _ => []
   end.
 
@@ -234,9 +238,10 @@ Fixpoint used_lifetime_vars_ty (T : Ty) : list nat :=
         | [] => env_indices ++ used_lifetime_vars_ty ret
         | x :: rest => used_lifetime_vars_ty x ++ go rest
         end
-      in go args
-  | MkTy _ (TForall _ _ body) => used_lifetime_vars_ty body
-  | MkTy _ (TRef (LVar i) _ inner) => i :: used_lifetime_vars_ty inner
+	      in go args
+	  | MkTy _ (TForall _ _ body) => used_lifetime_vars_ty body
+	  | MkTy _ (TTypeForall _ _ body) => used_lifetime_vars_ty body
+	  | MkTy _ (TRef (LVar i) _ inner) => i :: used_lifetime_vars_ty inner
   | MkTy _ (TRef _ _ inner) => used_lifetime_vars_ty inner
   | _ => []
   end.
